IsaSAT: more

Weidenbach_Book/IsaSAT_Rephase.thy
@@ -71,4 +71,93 @@ lemma rephase_random_spec:
   apply (auto dest: in_list_in_setD)
   done
 
+
+definition phase_save_rephase :: \<open>phase_save_heur \<Rightarrow> phase_save_heur nres\<close> where
+\<open>phase_save_rephase = (\<lambda>(\<phi>, target_assigned, target, best_assigned, best, end_of_phase, curr_phase).
+    if curr_phase = 0
+    then do {
+       \<phi> \<leftarrow> rephase_init False \<phi>;
+       RETURN (\<phi>, target_assigned, target, best_assigned, best, end_of_phase, 1)
+    }
+    else if curr_phase = 1
+    then do {
+       \<phi> \<leftarrow> copy_phase best \<phi>;
+       RETURN (\<phi>, target_assigned, target, best_assigned, best, end_of_phase, 2)
+    }
+    else if curr_phase = 2
+    then do {
+       \<phi> \<leftarrow> rephase_init True \<phi>;
+       RETURN (\<phi>, target_assigned, target, best_assigned, best, end_of_phase, 3)
+    }
+    else if curr_phase = 3
+    then do {
+       \<phi> \<leftarrow> rephase_random end_of_phase \<phi>;
+       RETURN (\<phi>, target_assigned, target, best_assigned, best, end_of_phase, 4)
+    }
+    else do {
+       \<phi> \<leftarrow> copy_phase best \<phi>;
+       RETURN (\<phi>, target_assigned, target, best_assigned, best, end_of_phase, 0)
+    })\<close>
+
+lemma phase_save_rephase_spec:
+  assumes \<open>phase_save_heur_rel \<A> \<phi>\<close>
+  shows \<open>phase_save_rephase \<phi> \<le> \<Down>Id (SPEC(phase_save_heur_rel \<A>))\<close>
+proof -
+  obtain \<phi>' target_assigned target best_assigned best end_of_phase curr_phase where
+    \<phi>: \<open>\<phi> = (\<phi>', target_assigned, target, best_assigned, best, end_of_phase, curr_phase)\<close>
+    by (cases \<phi>) auto
+  then have [simp]: \<open>length \<phi>' = length best\<close>
+    using assms by (auto simp: phase_save_heur_rel_def)
+  have 1: \<open>\<Down>Id (SPEC(phase_save_heur_rel \<A>)) \<ge>
+    \<Down>Id((\<lambda>(\<phi>, target_assigned, target, best_assigned, best, end_of_phase, curr_phase).
+      if curr_phase = 0 then  do {
+        \<phi>' \<leftarrow> SPEC (\<lambda>\<phi>'. length \<phi> = length \<phi>');
+        RETURN (\<phi>', target_assigned, target, best_assigned, best, end_of_phase, 1)
+      }
+     else if curr_phase = 1 then  do {
+        \<phi>' \<leftarrow> SPEC (\<lambda>\<phi>'. length \<phi> = length \<phi>');
+        RETURN (\<phi>', target_assigned, target, best_assigned, best, end_of_phase, 2)
+     }
+     else if curr_phase = 2 then  do {
+        \<phi>' \<leftarrow> SPEC (\<lambda>\<phi>'. length \<phi> = length \<phi>');
+        RETURN (\<phi>', target_assigned, target, best_assigned, best, end_of_phase, 3)
+     }
+     else if curr_phase = 3 then  do {
+        \<phi>' \<leftarrow> SPEC (\<lambda>\<phi>'. length \<phi> = length \<phi>');
+        RETURN (\<phi>', target_assigned, target, best_assigned, best, end_of_phase, 4)
+     }
+     else do {
+        \<phi>' \<leftarrow> SPEC (\<lambda>\<phi>'. length \<phi> = length \<phi>');
+        RETURN (\<phi>', target_assigned, target, best_assigned, best, end_of_phase, 0)
+     }) \<phi>)\<close>
+   using assms
+   by (cases \<phi>)
+    (auto simp: phase_save_heur_rel_def phase_saving_def RES_RETURN_RES)
+
+  show ?thesis
+    unfolding phase_save_rephase_def \<phi>
+    apply (simp only: prod.case)
+    apply (rule order_trans)
+    defer
+    apply (rule 1)
+    apply (simp only: prod.case \<phi>)
+    apply (refine_vcg if_mono rephase_init_spec copy_phase_spec rephase_random_spec)
+    apply (auto simp: phase_save_rephase_def)
+    done
+qed
+
+definition rephase_heur :: \<open>restart_heuristics \<Rightarrow> restart_heuristics nres\<close> where
+  \<open>rephase_heur = (\<lambda>(fast_ema, slow_ema, restart_info, wasted, \<phi>).
+    do {
+      \<phi> \<leftarrow> phase_save_rephase \<phi>;
+      RETURN (fast_ema, slow_ema, restart_info, wasted, \<phi>)
+   })\<close>
+
+lemma rephase_heur_spec:
+  \<open>heuristic_rel \<A> heur \<Longrightarrow> rephase_heur heur \<le>  \<Down>Id (SPEC(heuristic_rel \<A>))\<close>
+  unfolding rephase_heur_def
+  apply (refine_vcg phase_save_rephase_spec[THEN order_trans])
+  apply (auto simp: heuristic_rel_def)
+  done
+
 end
